src/spec/TLS13.ConnectionState.ProtectedWireSegmentation.fsti
@@ -146,6 +146,138 @@ let paired_replay_split_prefixes_equal
     Seq.equal server_prefix_sent client_prefix_received /\
     Seq.equal client_prefix_sent server_prefix_received
 
+noextract
+let paired_replay_split_prefixes_equal_with_full_streams
+  (server_model:CS.connection_model)
+  (client_model:CS.connection_model)
+  (server_prefix:list CS.conn_event)
+  (server_suffix:list CS.conn_event)
+  (client_prefix:list CS.conn_event)
+  (client_suffix:list CS.conn_event)
+  (server_full_sent:B.bytes)
+  (server_full_received:B.bytes)
+  (client_full_sent:B.bytes)
+  (client_full_received:B.bytes)
+  (server_final:CS.connection_model)
+  (client_final:CS.connection_model)
+  : prop =
+  forall
+    (server_mid:CS.connection_model)
+    (client_mid:CS.connection_model)
+    (server_prefix_sent:B.bytes)
+    (server_prefix_received:B.bytes)
+    (server_suffix_sent:B.bytes)
+    (server_suffix_received:B.bytes)
+    (client_prefix_sent:B.bytes)
+    (client_prefix_received:B.bytes)
+    (client_suffix_sent:B.bytes)
+    (client_suffix_received:B.bytes).
+    Seq.equal server_full_sent client_full_received /\
+    Seq.equal client_full_sent server_full_received /\
+    Seq.equal server_full_sent
+      (B.append server_prefix_sent server_suffix_sent) /\
+    Seq.equal server_full_received
+      (B.append server_prefix_received server_suffix_received) /\
+    Seq.equal client_full_sent
+      (B.append client_prefix_sent client_suffix_sent) /\
+    Seq.equal client_full_received
+      (B.append client_prefix_received client_suffix_received) /\
+    CS.conn_events_sent_seal_replay
+      server_model
+      server_prefix
+      server_prefix_sent
+      server_prefix_received
+      server_mid /\
+    CS.conn_events_sent_seal_replay
+      server_mid
+      server_suffix
+      server_suffix_sent
+      server_suffix_received
+      server_final /\
+    CS.conn_events_received_decode_replay
+      server_model
+      server_prefix
+      server_prefix_sent
+      server_prefix_received
+      server_mid /\
+    CS.conn_events_received_decode_replay
+      server_mid
+      server_suffix
+      server_suffix_sent
+      server_suffix_received
+      server_final /\
+    CS.conn_events_sent_seal_replay
+      client_model
+      client_prefix
+      client_prefix_sent
+      client_prefix_received
+      client_mid /\
+    CS.conn_events_sent_seal_replay
+      client_mid
+      client_suffix
+      client_suffix_sent
+      client_suffix_received
+      client_final /\
+    CS.conn_events_received_decode_replay
+      client_model
+      client_prefix
+      client_prefix_sent
+      client_prefix_received
+      client_mid /\
+    CS.conn_events_received_decode_replay
+      client_mid
+      client_suffix
+      client_suffix_sent
+      client_suffix_received
+      client_final ==>
+    Seq.equal server_prefix_sent client_prefix_received /\
+    Seq.equal client_prefix_sent server_prefix_received
+
+val lemma_paired_replay_split_prefixes_equal_from_full_streams
+  (server_model:CS.connection_model)
+  (client_model:CS.connection_model)
+  (server_prefix:list CS.conn_event)
+  (server_suffix:list CS.conn_event)
+  (client_prefix:list CS.conn_event)
+  (client_suffix:list CS.conn_event)
+  (server_full_sent:B.bytes)
+  (server_full_received:B.bytes)
+  (client_full_sent:B.bytes)
+  (client_full_received:B.bytes)
+  (server_final:CS.connection_model)
+  (client_final:CS.connection_model)
+  : Lemma
+      (requires
+        Seq.equal server_full_sent client_full_received /\
+        Seq.equal client_full_sent server_full_received /\
+        paired_replay_split_prefixes_equal_with_full_streams
+          server_model
+          client_model
+          server_prefix
+          server_suffix
+          client_prefix
+          client_suffix
+          server_full_sent
+          server_full_received
+          client_full_sent
+          client_full_received
+          server_final
+          client_final)
+      (ensures
+        paired_replay_split_prefixes_equal
+          server_model
+          client_model
+          server_prefix
+          server_suffix
+          client_prefix
+          client_suffix
+          server_full_sent
+          server_full_received
+          client_full_sent
+          client_full_received
+          server_final
+          client_final)
+
 val lemma_same_endpoint_replay_split_prefixes_equal_empty
   (model:CS.connection_model)
   (suffix:list CS.conn_event)
